format-version: 1.0
data-version: 1
date: 05:23:2016 03:00
saved-by: sgn
default-namespace: cxgn_time_ontology
remark: none
ontology: cxgn_time

[Term]
id: TIME:0000000
name: Time

[Term]
id: TIME:0000001
name: time of day
def: "Categorical day periods." []
is_a: TIME:0000000

[Term]
id: TIME:0000002
name: end of night
synonym: "EoN" EXACT []
def: "Half an hour before sunrise." []
is_a: TIME:0000001

[Term]
id: TIME:0000003
name: end of day
synonym: "EoD" EXACT []
def: "Late afternoon daylight." []
is_a: TIME:0000001

[Term]
id: TIME:0000004
name: mid day
synonym: "MD" EXACT []
def: "Between 11:00 in the morning and 14:00 in the afternoon." []
is_a: TIME:0000001

[Term]
id: TIME:0000005
name: time of year
def: "Days, weeks and months." []
is_a: TIME:0000000

[Term]
id: TIME:0000006
name: week 1
synonym: "Wk1" EXACT []
def: "" []
is_a: TIME:0000005

[Term]
id: TIME:0000007
name: week 2
synonym: "Wk2" EXACT []
def: "" []
is_a: TIME:0000005

[Term]
id: TIME:0000008
name: week 3
synonym: "Wk3" EXACT []
def: "" []
is_a: TIME:0000005

[Term]
id: TIME:0000009
name: week 4
synonym: "Wk4" EXACT []
def: "" []
is_a: TIME:0000005

[Term]
id: TIME:0000010
name: week 5
synonym: "Wk5" EXACT []
def: "" []
is_a: TIME:0000005

[Term]
id: TIME:0000011
name: week 6
synonym: "Wk6" EXACT []
def: "" []
is_a: TIME:0000005

[Term]
id: TIME:0000012
name: week 7
synonym: "Wk7" EXACT []
def: "" []
is_a: TIME:0000005

[Term]
id: TIME:0000013
name: week 8
synonym: "Wk8" EXACT []
def: "" []
is_a: TIME:0000005

[Term]
id: TIME:0000014
name: week 9
synonym: "Wk9" EXACT []
def: "" []
is_a: TIME:0000005

[Term]
id: TIME:0000015
name: week 10
synonym: "Wk10" EXACT []
def: "" []
is_a: TIME:0000005

[Term]
id: TIME:0000016
name: week 11
synonym: "Wk11" EXACT []
def: "" []
is_a: TIME:0000005

[Term]
id: TIME:0000017
name: week 12
synonym: "Wk12" EXACT []
def: "" []
is_a: TIME:0000005

[Term]
id: TIME:0000018
name: week 13
synonym: "Wk13" EXACT []
def: "" []
is_a: TIME:0000005

[Term]
id: TIME:0000019
name: week 14
synonym: "Wk14" EXACT []
def: "" []
is_a: TIME:0000005

[Term]
id: TIME:0000020
name: week 15
synonym: "Wk15" EXACT []
def: "" []
is_a: TIME:0000005

[Term]
id: TIME:0000021
name: week 16
synonym: "Wk16" EXACT []
def: "" []
is_a: TIME:0000005

[Term]
id: TIME:0000022
name: week 17
synonym: "Wk17" EXACT []
def: "" []
is_a: TIME:0000005

[Term]
id: TIME:0000023
name: week 18
synonym: "Wk18" EXACT []
def: "" []
is_a: TIME:0000005

[Term]
id: TIME:0000024
name: week 19
synonym: "Wk19" EXACT []
def: "" []
is_a: TIME:0000005

[Term]
id: TIME:0000025
name: week 20
synonym: "Wk20" EXACT []
def: "" []
is_a: TIME:0000005

[Term]
id: TIME:0000026
name: week 21
synonym: "Wk21" EXACT []
def: "" []
is_a: TIME:0000005

[Term]
id: TIME:0000027
name: week 22
synonym: "Wk22" EXACT []
def: "" []
is_a: TIME:0000005

[Term]
id: TIME:0000028
name: week 23
synonym: "Wk23" EXACT []
def: "" []
is_a: TIME:0000005

[Term]
id: TIME:0000029
name: week 24
synonym: "Wk24" EXACT []
def: "" []
is_a: TIME:0000005

[Term]
id: TIME:0000030
name: week 25
synonym: "Wk25" EXACT []
def: "" []
is_a: TIME:0000005

[Term]
id: TIME:0000031
name: week 26
synonym: "Wk26" EXACT []
def: "" []
is_a: TIME:0000005

[Term]
id: TIME:0000032
name: week 27
synonym: "Wk27" EXACT []
def: "" []
is_a: TIME:0000005

[Term]
id: TIME:0000033
name: week 28
synonym: "Wk28" EXACT []
def: "" []
is_a: TIME:0000005

[Term]
id: TIME:0000034
name: week 29
synonym: "Wk29" EXACT []
def: "" []
is_a: TIME:0000005

[Term]
id: TIME:0000035
name: week 30
synonym: "Wk30" EXACT []
def: "" []
is_a: TIME:0000005

[Term]
id: TIME:0000036
name: week 31
synonym: "Wk31" EXACT []
def: "" []
is_a: TIME:0000005

[Term]
id: TIME:0000037
name: week 32
synonym: "Wk32" EXACT []
def: "" []
is_a: TIME:0000005

[Term]
id: TIME:0000038
name: week 33
synonym: "Wk33" EXACT []
def: "" []
is_a: TIME:0000005

[Term]
id: TIME:0000039
name: week 34
synonym: "Wk34" EXACT []
def: "" []
is_a: TIME:0000005

[Term]
id: TIME:0000040
name: week 35
synonym: "Wk35" EXACT []
def: "" []
is_a: TIME:0000005

[Term]
id: TIME:0000041
name: week 36
synonym: "Wk36" EXACT []
def: "" []
is_a: TIME:0000005

[Term]
id: TIME:0000042
name: week 37
synonym: "Wk37" EXACT []
def: "" []
is_a: TIME:0000005

[Term]
id: TIME:0000043
name: week 38
synonym: "Wk38" EXACT []
def: "" []
is_a: TIME:0000005

[Term]
id: TIME:0000044
name: week 39
synonym: "Wk39" EXACT []
def: "" []
is_a: TIME:0000005

[Term]
id: TIME:0000045
name: week 40
synonym: "Wk40" EXACT []
def: "" []
is_a: TIME:0000005

[Term]
id: TIME:0000046
name: week 41
synonym: "Wk41" EXACT []
def: "" []
is_a: TIME:0000005

[Term]
id: TIME:0000047
name: week 42
synonym: "Wk42" EXACT []
def: "" []
is_a: TIME:0000005

[Term]
id: TIME:0000048
name: week 43
synonym: "Wk43" EXACT []
def: "" []
is_a: TIME:0000005

[Term]
id: TIME:0000049
name: week 44
synonym: "Wk44" EXACT []
def: "" []
is_a: TIME:0000005

[Term]
id: TIME:0000050
name: week 45
synonym: "Wk45" EXACT []
def: "" []
is_a: TIME:0000005

[Term]
id: TIME:0000051
name: week 46
synonym: "Wk46" EXACT []
def: "" []
is_a: TIME:0000005

[Term]
id: TIME:0000052
name: week 47
synonym: "Wk47" EXACT []
def: "" []
is_a: TIME:0000005

[Term]
id: TIME:0000053
name: week 48
synonym: "Wk48" EXACT []
def: "" []
is_a: TIME:0000005

[Term]
id: TIME:0000054
name: week 49
synonym: "Wk49" EXACT []
def: "" []
is_a: TIME:0000005

[Term]
id: TIME:0000055
name: week 50
synonym: "Wk50" EXACT []
def: "" []
is_a: TIME:0000005

[Term]
id: TIME:0000056
name: week 51
synonym: "Wk51" EXACT []
def: "" []
is_a: TIME:0000005

[Term]
id: TIME:0000057
name: week 52
synonym: "Wk52" EXACT []
def: "" []
is_a: TIME:0000005

[Term]
id: TIME:0000058
name: week 53
synonym: "Wk53" EXACT []
def: "" []
is_a: TIME:0000005

[Term]
id: TIME:0000059
name: week 54
synonym: "Wk54" EXACT []
def: "" []
is_a: TIME:0000005

[Term]
id: TIME:0000060
name: month 1
synonym: "Mo1" EXACT []
def: "" []
is_a: TIME:0000005

[Term]
id: TIME:0000061
name: month 2
synonym: "Mo2" EXACT []
def: "" []
is_a: TIME:0000005

[Term]
id: TIME:0000062
name: month 3
synonym: "Mo3" EXACT []
def: "" []
is_a: TIME:0000005

[Term]
id: TIME:0000063
name: month 4
synonym: "Mo4" EXACT []
def: "" []
is_a: TIME:0000005

[Term]
id: TIME:0000064
name: month 5
synonym: "Mo5" EXACT []
def: "" []
is_a: TIME:0000005

[Term]
id: TIME:0000065
name: month 6
synonym: "Mo6" EXACT []
def: "" []
is_a: TIME:0000005

[Term]
id: TIME:0000066
name: month 7
synonym: "Mo7" EXACT []
def: "" []
is_a: TIME:0000005

[Term]
id: TIME:0000067
name: month 8
synonym: "Mo8" EXACT []
def: "" []
is_a: TIME:0000005

[Term]
id: TIME:0000068
name: month 9
synonym: "Mo9" EXACT []
def: "" []
is_a: TIME:0000005

[Term]
id: TIME:0000069
name: month 10
synonym: "Mo10" EXACT []
def: "" []
is_a: TIME:0000005

[Term]
id: TIME:0000070
name: month 11
synonym: "Mo11" EXACT []
def: "" []
is_a: TIME:0000005

[Term]
id: TIME:0000071
name: month 12
synonym: "Mo12" EXACT []
def: "" []
is_a: TIME:0000005

[Term]
id: TIME:0000076
name: "categorical plant stage"
def: "." []
is_a: TIME:0000000

[Term]
id: TIME:0000077
name: at flowering
synonym: "FLW" EXACT []
def: "flowering (shooting is here equivalent to flowering) stage"
is_a: TIME:0000076

[Term]
id: TIME:0000078
name: at harvesting
synonym: "HVT" EXACT []
def: "harvesting stage"
is_a: TIME:0000076

[Term]
id: TIME:0000079
name: at post-harvesting
synonym: "PHVT" EXACT []
def: "post harvesting stage"
is_a: TIME:0000076

[Term]
id: TIME:0000080
name: at planting
synonym: "PLT" EXACT []
def: "planting stage:
is_a: TIME:0000076

[Term]
id: TIME:0000081
name: date of
synonym: "DCOL" EXACT []
def: "date of data collection (dd/mm/yyyy)"
is_a: TIME:0000076

[Term]
id: TIME:0000082
name: day 1
synonym: "D01" EXACT []
def: "" []
is_a: TIME:0000005

[Term]
id: TIME:0000083
name: day 2
synonym: "D02" EXACT []
def: "" []
is_a: TIME:0000005

[Term]
id: TIME:0000084
name: day 3
synonym: "D03" EXACT []
def: "" []
is_a: TIME:0000005

[Term]
id: TIME:0000085
name: day 4
synonym: "D04" EXACT []
def: "" []
is_a: TIME:0000005

[Term]
id: TIME:0000086
name: day 5
synonym: "D05" EXACT []
def: "" []
is_a: TIME:0000005

[Term]
id: TIME:0000087
name: day 6
synonym: "D06" EXACT []
def: "" []
is_a: TIME:0000005

[Term]
id: TIME:0000088
name: day 7
synonym: "D07" EXACT []
def: "" []
is_a: TIME:0000005

[Term]
id: TIME:0000089
name: day 8
synonym: "D08" EXACT []
def: "" []
is_a: TIME:0000005

[Term]
id: TIME:0000090
name: day 9
synonym: "D09" EXACT []
def: "" []
is_a: TIME:0000005

[Term]
id: TIME:0000091
name: day 10
synonym: "D10" EXACT []
def: "" []
is_a: TIME:0000005

[Term]
id: TIME:0000092
name: day 11
synonym: "D11" EXACT []
def: "" []
is_a: TIME:0000005

[Term]
id: TIME:0000093
name: day 12
synonym: "D12" EXACT []
def: "" []
is_a: TIME:0000005

[Term]
id: TIME:0000094
name: day 13
synonym: "D13" EXACT []
def: "" []
is_a: TIME:0000005

[Term]
id: TIME:0000095
name: day 14
synonym: "D14" EXACT []
def: "" []
is_a: TIME:0000005

[Term]
id: TIME:0000096
name: day 15
synonym: "D15" EXACT []
def: "" []
is_a: TIME:0000005

[Term]
id: TIME:0000097
name: day 16
synonym: "D16" EXACT []
def: "" []
is_a: TIME:0000005

[Term]
id: TIME:0000098
name: day 17
synonym: "D17" EXACT []
def: "" []
is_a: TIME:0000005

[Term]
id: TIME:0000099
name: day 18
synonym: "D18" EXACT []
def: "" []
is_a: TIME:0000005

[Term]
id: TIME:0000100
name: day 19
synonym: "D19" EXACT []
def: "" []
is_a: TIME:0000005

[Term]
id: TIME:0000101
name: day 20
synonym: "D20" EXACT []
def: "" []
is_a: TIME:0000005

[Term]
id: TIME:0000102
name: day 21
synonym: "D21" EXACT []
def: "" []
is_a: TIME:0000005

[Term]
id: TIME:0000103
name: day 22
synonym: "D22" EXACT []
def: "" []
is_a: TIME:0000005

[Term]
id: TIME:0000104
name: day 23
synonym: "D23" EXACT []
def: "" []
is_a: TIME:0000005

[Term]
id: TIME:0000105
name: day 24
synonym: "D24" EXACT []
def: "" []
is_a: TIME:0000005

[Term]
id: TIME:0000106
name: day 25
synonym: "D25" EXACT []
def: "" []
is_a: TIME:0000005

[Term]
id: TIME:0000107
name: day 26
synonym: "D26" EXACT []
def: "" []
is_a: TIME:0000005

[Term]
id: TIME:0000108
name: day 27
synonym: "D27" EXACT []
def: "" []
is_a: TIME:0000005

[Term]
id: TIME:0000109
name: day 28
synonym: "D28" EXACT []
def: "" []
is_a: TIME:0000005

[Term]
id: TIME:0000110
name: day 29
synonym: "D29" EXACT []
def: "" []
is_a: TIME:0000005

[Term]
id: TIME:0000111
name: day 30
synonym: "D30" EXACT []
def: "" []
is_a: TIME:0000005

[Term]
id: TIME:0000112
name: day 31
synonym: "D31" EXACT []
def: "" []
is_a: TIME:0000005

[Term]
id: TIME:0000113
name: hour 1
synonym: "H01" EXACT []
def: "" []
is_a: TIME:0000005

[Term]
id: TIME:0000114
name: hour 2
synonym: "H02" EXACT []
def: "" []
is_a: TIME:0000005

[Term]
id: TIME:0000115
name: hour 3
synonym: "H03" EXACT []
def: "" []
is_a: TIME:0000005

[Term]
id: TIME:0000116
name: hour 4
synonym: "H04" EXACT []
def: "" []
is_a: TIME:0000005

[Term]
id: TIME:0000117
name: hour 5
synonym: "H05" EXACT []
def: "" []
is_a: TIME:0000005

[Term]
id: TIME:0000118
name: hour 6
synonym: "H06" EXACT []
def: "" []
is_a: TIME:0000005

[Term]
id: TIME:0000119
name: hour 7
synonym: "H07" EXACT []
def: "" []
is_a: TIME:0000005

[Term]
id: TIME:0000120
name: hour 8
synonym: "H08" EXACT []
def: "" []
is_a: TIME:0000005

[Term]
id: TIME:0000121
name: hour 9
synonym: "H09" EXACT []
def: "" []
is_a: TIME:0000005

[Term]
id: TIME:0000122
name: hour 10
synonym: "H10" EXACT []
def: "" []
is_a: TIME:0000005

[Term]
id: TIME:0000123
name: hour 11
synonym: "H11" EXACT []
def: "" []
is_a: TIME:0000005

[Term]
id: TIME:0000124
name: hour 12
synonym: "H12" EXACT []
def: "" []
is_a: TIME:0000005

[Term]
id: TIME:0000125
name: hour 13
synonym: "H13" EXACT []
def: "" []
is_a: TIME:0000005

[Term]
id: TIME:0000126
name: hour 14
synonym: "H14" EXACT []
def: "" []
is_a: TIME:0000005

[Term]
id: TIME:0000127
name: hour 15
synonym: "H15" EXACT []
def: "" []
is_a: TIME:0000005

[Term]
id: TIME:0000128
name: hour 16
synonym: "H16" EXACT []
def: "" []
is_a: TIME:0000005

[Term]
id: TIME:0000129
name: hour 17
synonym: "H17" EXACT []
def: "" []
is_a: TIME:0000005

[Term]
id: TIME:0000130
name: hour 18
synonym: "H18" EXACT []
def: "" []
is_a: TIME:0000005

[Term]
id: TIME:0000131
name: hour 19
synonym: "H19" EXACT []
def: "" []
is_a: TIME:0000005

[Term]
id: TIME:0000132
name: hour 20
synonym: "H20" EXACT []
def: "" []
is_a: TIME:0000005

[Term]
id: TIME:0000133
name: hour 21
synonym: "H21" EXACT []
def: "" []
is_a: TIME:0000005

[Term]
id: TIME:0000134
name: hour 22
synonym: "H22" EXACT []
def: "" []
is_a: TIME:0000005

[Term]
id: TIME:0000135
name: hour 23
synonym: "H23" EXACT []
def: "" []
is_a: TIME:0000005

[Term]
id: TIME:0000136
name: hour 24
synonym: "H24" EXACT []
def: "" []
is_a: TIME:0000005

[Term]
id: TIME:0000137
name: at maiden
synonym: "MAD" EXACT []
def: "maiden stage:
is_a: TIME:0000076

[Term]
id: TIME:0000080
name: at pre-flowering
synonym: "PFL" EXACT []
def: "pre-flowering stage:
is_a: TIME:0000076
